@prefix rdf: <http://www.w3.org/1999/02/22-rdf-syntax-ns#> .
@prefix rdfs: <http://www.w3.org/2000/01/rdf-schema#> .
@prefix owl: <http://www.w3.org/2002/07/owl#> .
@prefix xsd: <http://www.w3.org/2001/XMLSchema#> .
@prefix foaf: <http://xmlns.com/foaf/0.1/> .
@prefix dct: <http://purl.org/dc/terms/> .
@prefix prov: <http://www.w3.org/ns/prov#> .
@prefix : <http://mobi.com/ontologies/prov#> .
@base <http://mobi.com/ontologies/prov> .

<http://mobi.com/ontologies/prov> a owl:Ontology ;
    owl:versionIRI <http://mobi.com/ontologies/prov#1.0> ;
    owl:imports <http://www.w3.org/ns/prov#> ;
    rdfs:label "The Mobi Provenance Ontology"@en ;
    rdfs:comment "The Mobi Provenance ontology describes specific types of PROV-O Activities for the application."@en;
    dct:creator [foaf:name "Megan Mercer"] ;
    foaf:maker [foaf:name "Mobi"; foaf:homepage <https://mobi.inovexcorp.com/>] ;
    dct:modified "2017-08-02"^^xsd:date .

:actionWord a owl:AnnotationProperty, owl:FunctionalProperty;
    rdfs:domain prov:Activity;
    dct:title "Activity Action"@en ;
    dct:description "The action word associated with the Activity type"@en .
    
:provAction a owl:ObjectProperty, owl:FunctionalProperty;
    rdfs:domain prov:Activity;
    dct:title "Prov Action"@en ;
    dct:description "The prov action associated with the Activity type"@en .

# CreateActivity

:CreateActivity a owl:Class ;
    rdfs:subClassOf prov:Activity ;
    :actionWord "created"@en ;
    :provAction prov:generated ;
    dct:title "Create Activity"@en ;
    dct:description "A CreateActivity represents an event that caused the creation of a new resource. An example would be creating a new Record."@en .

# DeleteActivity

:DeleteActivity a owl:Class ;
    rdfs:subClassOf prov:Activity ;
    :actionWord "deleted"@en;
    :provAction prov:invalidated ;
    dct:title "Delete Activity"@en ;
    dct:description "A DeleteActivity represents an event that caused the deletion of a resource. An example would be deleting a Record."@en .

# UpdateActivity

:UpdateActivity a owl:Class ;
    rdfs:subClassOf prov:Activity ;
    :actionWord "updated"@en;
    :provAction prov:used ;
    dct:title "Update Activity"@en ;
    dct:description "An UpdateActivity represents an event that caused a resource to be updated. An example would be when a Record's metadata is updated."@en .

# UseActivity

:UseActivity a owl:Class ;
    rdfs:subClassOf prov:Activity ;
    :actionWord "used"@en;
    :provAction prov:used ;
    dct:title "Utilization Activity"@en ;
    dct:description "A UseActivity represents an event where a resource was utilized in some process. An example would be when a Mapping is run against some data."@en .

# SystemActivity

:SystemActivity a owl:Class ;
    rdfs:subClassOf prov:Activity ;
    :actionWord "interacted with"@en;
    :provAction prov:used ;
    dct:title "System Activity"@en ;
    dct:description "A SystemActivity represents an event relating to the application as a whole. Examples would be when a user logs in or data is uploaded through the admin command line."@en .