@prefix rdf: <http://www.w3.org/1999/02/22-rdf-syntax-ns#>.
@prefix owl: <http://www.w3.org/2002/07/owl#>.
@prefix xsd: <http://www.w3.org/2001/XMLSchema#>.
@prefix rdfs: <http://www.w3.org/2000/01/rdf-schema#>.
@prefix dct: <http://purl.org/dc/terms/>.
@prefix foaf: <http://xmlns.com/foaf/0.1/>.
@prefix muser: <http://mobi.com/ontologies/user/management#> .
@prefix mobi: <http://mobi.com/ontologies/mobi#> .
@prefix : <http://mobi.com/ontologies/platform/config#>.
@base <http://mobi.com/ontologies/platform/config>.

<http://mobi.com/ontologies/platform/config> a owl:Ontology;
    owl:versionIRI <http://mobi.com/ontologies/platform/config/1.0>;
    owl:imports <http://mobi.com/ontologies/user/management>, <http://mobi.com/ontologies/matonto> ;
    rdfs:label "The Mobi platform configuration ontology"@en;
    rdfs:comment "The Mobi platform configuration ontology describes how user preferences, user state, and applications are expressed within the Mobi framework."@en;
    dct:creator [foaf:name "Jordan Lewis"], [foaf:name "Megan Mercer"], [foaf:name "Stephen Kahmann"];
    foaf:maker [foaf:name "Mobi"; foaf:homepage <https://mobi.inovexcorp.com/>];
    dct:modified "2017-10-06"^^xsd:date.

# Application

:Application a owl:Class;
    rdfs:label "Application"@en;
    rdfs:comment "A representative of an application in Mobi."@en.

# State

:State a owl:Class;
    rdfs:label "State"@en;
    rdfs:comment "A representative of a user's last state for an aspect of Mobi."@en.

:stateResource a owl:ObjectProperty;
    rdfs:label "state resource"@en;
    rdfs:comment "The subject of one of the resources associated with the described State."@en;
    rdfs:domain :State;
    rdfs:range mobi:Identifier.

# ApplicationState

:ApplicationState a owl:Class;
    rdfs:subClassOf :State;
    rdfs:label "Application State"@en;
    rdfs:comment "A representation of a user's last state for a specific application in Mobi."@en.

:application a owl:ObjectProperty, owl:FunctionalProperty;
    rdfs:label "application"@en;
    rdfs:comment "The Application associated with the described ApplicationState."@en;
    rdfs:domain :ApplicationState;
    rdfs:range :Application.

# Preferences

:Preferences a owl:Class;
    rdfs:label "Preferences"@en;
    rdfs:comment "A set of key-value pairs representing preferences a User has chosen."@en.

# Ontology Preferences

:OntologyPreferences a owl:Class;
    rdfs:subClassOf :Preferences;
    rdfs:label "Ontology Preferences"@en;
    rdfs:comment "The set of Ontology Editor preferences that a User has chosen."@en.

:dropDownTooltipDisplay a owl:DatatypeProperty, owl:FunctionalProperty;
    rdfs:label "drop down tooltip display"@en;
    rdfs:comment "The display type shown when you hover over items in dropdown fields in the Ontology Editor."@en;
    rdfs:domain :OntologyPreferences;
    rdfs:range rdfs:Literal.

:treeItemDisplay a owl:DatatypeProperty, owl:FunctionalProperty;
    rdfs:label "tree item display"@en;
    rdfs:comment "The display type shown in tree views in the Ontology Editor."@en;
    rdfs:domain :OntologyPreferences;
    rdfs:range rdfs:Literal.

# Misc.

:forUser a owl:ObjectProperty, owl:FunctionalProperty;
    rdfs:label "for user"@en;
    rdfs:comment "The User associated with the described Preferences or State."@en;
    # ORM issue with blank node domains. Will show up on ontology _Thing
    #rdfs:domain [a owl:Class; owl:unionOf(:State :Preferences)];
    rdfs:range muser:User.