@prefix : <http://matonto.org/ontologies/delimited#> .
@prefix owl: <http://www.w3.org/2002/07/owl#> .
@prefix rdf: <http://www.w3.org/1999/02/22-rdf-syntax-ns#> .
@prefix xml: <http://www.w3.org/XML/1998/namespace> .
@prefix xsd: <http://www.w3.org/2001/XMLSchema#> .
@prefix rdfs: <http://www.w3.org/2000/01/rdf-schema#> .
@prefix mcat: <http://matonto.org/ontologies/catalog#> .

<http://matonto.org/ontologies/delimited> a owl:Ontology ;
    owl:imports <http://matonto.org/ontologies/catalog> ;
    owl:versionIRI <http://matonto.org/ontologies/delimited#1.1>;
    rdfs:label "Delimited" ;
    rdfs:comment "An ontology which defines MatOnto Mappings." .

#################################################################
#
#    Object Properties
#
#################################################################

###  http://matonto.org/ontologies/delimited#classMapping

:classMapping a owl:ObjectProperty ;
    rdfs:domain :ObjectMapping ;
    rdfs:range :ClassMapping ;
    rdfs:label "class mapping" ;
    rdfs:comment "The ClassMapping that describes the target resource." .

###  http://matonto.org/ontologies/delimited#dataProperty

:dataProperty a owl:ObjectProperty ;
    rdfs:subPropertyOf :propertyMapping ;
    rdfs:domain :ClassMapping ;
    rdfs:range :DataMapping ;
    rdfs:label "data property" ;
    rdfs:comment "A data property mapping for a ClassMapping." .

###  http://matonto.org/ontologies/delimited#hasProperty

:hasProperty a owl:ObjectProperty ;
	rdfs:domain :DataMapping , :ObjectMapping , :PropertyMapping ;
	rdfs:range rdf:Property ;
    rdfs:label "has property" ;
	rdfs:comment "The Property defines the relationship for the PropertyMapping" .

###  http://matonto.org/ontologies/delimited#mapsTo

:mapsTo a owl:ObjectProperty ;
    rdfs:domain :ClassMapping ;
    rdfs:range owl:Thing ;
    rdfs:label "maps to" ;
    rdfs:comment "Defines the type that will be used when defining an object from this class mapping" .

###  http://matonto.org/ontologies/delimited#objectProperty

:objectProperty a owl:ObjectProperty ;
    rdfs:subPropertyOf :propertyMapping ;
    rdfs:domain :ClassMapping ;
    rdfs:range :ObjectMapping ;
    rdfs:label "object property" ;
    rdfs:comment "An object property mapping for a ClassMapping." .

###  http://matonto.org/ontologies/delimited#propertyMapping

:propertyMapping a owl:ObjectProperty ;
    rdfs:range :PropertyMapping ;
    rdfs:label "property mapping" ;
    rdfs:comment "A property mapping, either data or object, for a ClassMapping." .

###  http://matonto.org/ontologies/delimited#sourceOntology

:sourceOntology a owl:ObjectProperty, owl:FunctionalProperty ;
    rdfs:domain :Mapping ;
    rdfs:range owl:Ontology ;
    rdfs:label "source ontology" ;
    rdfs:comment "Defines the ontology that the Mapping is based on." .

###  http://matonto.org/ontologies/delimited#sourceOntologyRecord

:sourceRecord a owl:ObjectProperty, owl:FunctionalProperty ;
    rdfs:domain :Mapping ;
    rdfs:range mcat:OntologyRecord ;
    rdfs:label "source record" ;
    rdfs:comment "Defines the OntologyRecord that the Mapping is based on." .

###  http://matonto.org/ontologies/delimited#sourceBranch

:sourceBranch a owl:ObjectProperty, owl:FunctionalProperty ;
    rdfs:domain :Mapping ;
    rdfs:range mcat:Branch ;
    rdfs:label "source branch" ;
    rdfs:comment "Defines the Branch of the OntologyRecord that the Mapping is based on." .

###  http://matonto.org/ontologies/delimited#sourceCommit

:sourceCommit a owl:ObjectProperty, owl:FunctionalProperty ;
    rdfs:domain :Mapping ;
    rdfs:range mcat:Commit ;
    rdfs:label "source commit" ;
    rdfs:comment "Defines the Commit of the OntologyRecord that the Mapping is based on." .

###  http://matonto.org/ontologies/delimited#versionIRI

:versionIRI a owl:ObjectProperty, owl:FunctionalProperty ;
    rdfs:domain :Mapping ;
    rdfs:range xsd:anyURI ;
    rdfs:label "version IRI" ;
    rdfs:comment "The IRI of the current version of a Mapping." .

#################################################################
#
#    Data properties
#
#################################################################

###  http://matonto.org/ontologies/delimited#columnIndex

:columnIndex a owl:DatatypeProperty ;
    rdfs:domain :Cell , :DataMapping , :ObjectMapping ;
    rdfs:range xsd:integer ;
    rdfs:label "column index" ;
    rdfs:comment "The cells column. Starting at 0." .

###  http://matonto.org/ontologies/delimited#dataStart

:dataStart a owl:DatatypeProperty ;
    rdfs:domain :Document ;
    rdfs:range xsd:integer ;
    rdfs:label "data start" ;
    rdfs:comment "The row that the data starts. Used to avoid parsing headers incorrectly" .

###  http://matonto.org/ontologies/delimited#defaultPrefix

:defaultPrefix a owl:DatatypeProperty ;
    rdfs:subPropertyOf owl:topDataProperty ;
    rdfs:domain :Mapping ;
    rdfs:range xsd:string ;
    rdfs:label "default prefix" ;
    rdfs:comment "The default prefix used for the Mapping" .

###  http://matonto.org/ontologies/delimited#hasPrefix

:hasPrefix a owl:DatatypeProperty ;
    rdfs:domain :ClassMapping ;
    rdfs:range xsd:string ;
    rdfs:label "has prefix" ;
    rdfs:comment "The prefix used if the Cell is an instance" .

###  http://matonto.org/ontologies/delimited#localName

:localName a owl:DatatypeProperty, owl:FunctionalProperty ;
    rdfs:domain :ClassMapping ;
    rdfs:range xsd:string ;
    rdfs:label "local name" ;
    rdfs:comment "The pattern specifying the local name of the generated instance. A value of \"${UUID}\" results in the generation of random UUID. A digit value results in the value for the cell in that column being inserted into the IRI (e.g. ${2} would be the value for the third column in the row)" .

###  http://matonto.org/ontologies/delimited#quoteCharacter

:quoteCharacter a owl:DatatypeProperty ;
    rdfs:domain :Mapping ;
    rdfs:range xsd:string ;
    rdfs:label "quote character" ;
    rdfs:comment "The character used as quotes for cells" .

###  http://matonto.org/ontologies/delimited#separator

:separator a owl:DatatypeProperty ;
    rdfs:domain :Mapping ;
    rdfs:range xsd:string ;
    rdfs:label "separator" ;
    rdfs:comment "The character used as separator or delimiter between files columns" .


#################################################################
#
#    Classes
#
#################################################################


###  http://matonto.org/ontologies/delimited#ClassMapping

:ClassMapping a owl:Class ;
    rdfs:label "Class Mapping" ;
    rdfs:comment "An object that represents the creation of a specific type of individual." .

###  http://matonto.org/ontologies/delimited#DataMapping

:DataMapping a owl:Class ;
    rdfs:subClassOf :PropertyMapping ;
    rdfs:label "Data Mapping" ;
    rdfs:comment "An object used to relate a ClassMapping to a Datatype Property on the generated instance." .

###  http://matonto.org/ontologies/delimited#Mapping

:Mapping rdf:type owl:Class ;
    rdfs:label "Mapping" ;
    rdfs:comment "An object that represents a mapping configuration." .

###  http://matonto.org/ontologies/delimited#ObjectMapping

:ObjectMapping a owl:Class ;
    rdfs:subClassOf :PropertyMapping ;
    rdfs:label "Object Mapping" ;
    rdfs:comment "An object used to relate a ClassMapping to an Object Property on the generated instance." .

###  http://matonto.org/ontologies/delimited#PropertyMapping

:PropertyMapping a owl:Class ;
    rdfs:label "Property Mapping" ;
    rdfs:comment "An object used to relate a ClassMapping to a property on the generated instance." .

###  http://www.w3.org/1999/02/22-rdf-syntax-ns#Property

rdf:Property a owl:Class .
