@prefix rdf: <http://www.w3.org/1999/02/22-rdf-syntax-ns#> .
@prefix rdfs: <http://www.w3.org/2000/01/rdf-schema#> .
@prefix owl: <http://www.w3.org/2002/07/owl#> .
@prefix xsd: <http://www.w3.org/2001/XMLSchema#> .
@prefix foaf: <http://xmlns.com/foaf/0.1/> .
@prefix dct: <http://purl.org/dc/terms/> .
@prefix delim: <http://matonto.org/ontologies/delim#> .
@prefix dataset: <http://matonto.org/ontologies/dataset#> .
@prefix : <http://matonto.org/ontologies/etl#> .
@base <http://matonto.org/ontologies/etl> .

<http://matonto.org/ontologies/etl> a owl:Ontology ;
    owl:versionIRI <http://matonto.org/ontologies/etl#1.0> ;
    dct:title "The Mobi ETL Ontology"@en ;
    dct:creator [foaf:name "Megan Mercer"] ;
    foaf:maker [foaf:name "MatOnto"; foaf:homepage <http://matonto.org>] ;
    dct:modified "2017-08-22"^^xsd:date .

# Workflow

:Workflow a owl:Class ;
    dct:title "Workflow"@en ;
    dct:description "A Workflow defines a set of Routes which link DataSources, Processors, and Destinations together to perform data processing."@en .

:route a owl:ObjectProperty ;
    dct:title "route"@en ;
    dct:description "A Route in the described Workflow represented as an rdf:List which supports branching if need be. The Route must begin with a single DataSource and each branch must end in a Destination."@en ;
    rdfs:domain :Workflow ;
    rdfs:range rdf:List .

:dataSource a owl:ObjectProperty ;
    dct:title "data source"@en ;
    dct:description "A DataSource of the described Workflow."@en ;
    rdfs:domain :Workflow ;
    rdfs:range :DataSource .

:processor a owl:ObjectProperty ;
    dct:title "processor"@en ;
    dct:description "A Processor used in the described Workflow."@en ;
    rdfs:domain :Workflow ;
    rdfs:range :Processor .

:destination a owl:ObjectProperty ;
    dct:title "destination"@en ;
    dct:description "A Destination used in the described Workflow."@en ;
    rdfs:domain :Workflow ;
    rdfs:range :Destination .

# DataSource

:DataSource a owl:Class ;
    dct:title "Data Source"@en ;
    dct:description "A DataSource represents a configuration for retrieving data. This could be from a file system, the web, a database, etc. They are the starting points for Workflows."@en .

:FileDataSource a owl:Class ;
    rdfs:subClassOf :DataSource ;
    :outputType :FileMessage ;
    dct:title "File Data Source"@en ;
    dct:description "A FileDataSource provides configurations for retrieving a single file from a file system. Returns a FileMessage pointing to the specified file."@en .

:DirectoryDataSource a owl:Class ;
    rdfs:subClassOf :DataSource ;
    :outputType :FileMessage ;
    dct:title "Directory Data Source"@en ;
    dct:description "A DirectoryDataSource provides configurations for retrieving a directory of files from a file system. Returns FileMessages for each file found in the specified directory."@en .

:filter a owl:DatatypeProperty, owl:FunctionalProperty ;
    dct:title "filter"@en ;
    dct:description "A glob pattern to filter which files are collected from the described DirectoryDataSource."@en ;
    rdfs:domain :DirectoryDataSource ;
    rdfs:range xsd:string .

:recursive a owl:DatatypeProperty, owl:FunctionalProperty ;
    dct:title "recursive"@en ;
    dct:description "Whether or not the described DirectoryDataSource should collect files recursively. Default is false."@en ;
    rdfs:domain :DirectoryDataSource ;
    rdfs:range xsd:boolean .

# Processor

:Processor a owl:Class ;
    dct:title "Processor"@en ;
    dct:description "A Processor takes data as input and performs some act of processing to output to either another Processor or a Destination to end a Workflow. This could be a Mobi Mapping, an indexer, or other transformation services."@en .

:processTimeLimit a owl:DatatypeProperty, owl:FunctionalProperty ;
    dct:title "process time limit"@en ;
    dct:description "The limit in milliseconds for how long the described Processor should run. If not set, the time limit is infinite."@en ;
    rdfs:domain :Processor ;
    rdfs:range xsd:integer .

:MappingProcessor a owl:Class ;
    rdfs:subClassOf :Processor ;
    :inputType :FileMessage ;
    :outputType :RDFMessage ;
    dct:title "Mapping Processor"@en ;
    dct:description "A MappingProcessor provides configurations for running a Mobi Mapping against a set of data. Expects FileMessages pointing to SV or Excel files with tabular data. Outputs RDFMessages."@en .

:mappingRecord a owl:ObjectProperty, owl:FunctionalProperty ;
    dct:title "mapping record"@en ;
    dct:description "The MappingRecord that the described MappingProcessor uses to transform data."@en ;
    rdfs:domain :MappingProcessor ;
    rdfs:range delim:MappingRecord .

:containsHeaders a owl:DatatypeProperty, owl:FunctionalProperty ;
    dct:title "contains headers"@en ;
    dct:description "Whether or not the file(s) being processed by the described MappingProcessor have a header row."@en ;
    rdfs:domain :MappingProcessor ;
    rdfs:range xsd:boolean .

:separator a owl:DatatypeProperty, owl:FunctionalProperty ;
    dct:title "contains headers"@en ;
    dct:description "The character used to separate columns in SV file(s) processed by the described MappingProcessor"@en ;
    rdfs:domain :MappingProcessor ;
    rdfs:range xsd:string .

:TikaProcessor a owl:Class ;
    rdfs:subClassOf :Processor ;
    :inputType :FileMessage ;
    :outputType :FileMessage ;
    dct:title "Tika Processor"@en ;
    dct:description "A TikaProcessor provides configurations for retrieving metadata about and the string contents of a file. Expects FileMessages. Returns TikaMessages pointing to the created RDF and the string contents."@en .

:UnstructuredProcessor a owl:Class ;
    rdfs:subClassOf :Processor ;
    :inputType :FileMessage ;
    :outputType :RDFMessage ;
    dct:title "Unstructured Processor"@en ;
    dct:description "A UnstructuredProcessor provides configurations for running a file through the Mobi Unstructured Service to link referenced entities in a dataset to a document. Expects FileMessages. Returns RDFMessages."@en .

:lookupType a owl:ObjectProperty, owl:FunctionalProperty ;
    dct:title "lookup type"@en ;
    dct:description "The class whose instances will be searched for in the FileMessgae passed to the described UnstructuredProcessor."@en ;
    rdfs:domain :UnstructuredProcessor ;
    rdfs:range owl:Class .

:lookupProperty a owl:ObjectProperty ;
    dct:title "lookup property"@en ;
    dct:description "The property whose values on instances will be searched for in the FileMessage passed to the described UnstructuredProcessor."@en ;
    rdfs:domain :UnstructuredProcessor ;
    rdfs:range rdf:Property .

# Destination

:Destination a owl:Class ;
    dct:title "Destination"@en ;
    dct:description "A Destination is the end of a branch of processing in a Workflow and is intended to output the data into some sort of store. This could be a database, triple store, file, etc."@en .

:FileDestination a owl:Class ;
    rdfs:subClassOf :Destination ;
    :inputType :SerializableMessage ;
    dct:title "File Destination"@en ;
    dct:description "A FileDestination provides configurations for outputing data into a file on a file system."@en .

:DirectoryDestination a owl:Class ;
    rdfs:subClassOf :Destination ;
    :inputType :SerializableMessage ;
    dct:title "Directory Destination"@en ;
    dct:description "A DirectoryDestination provides configurations for outputing data into multiple files in a directory on a file system."@en .

:fileName a owl:DatatypeProperty, owl:FunctionalProperty ;
    dct:title "file name"@en ;
    dct:description "An expression to create the file name of a file saved by the described DirectoryDestination."@en ;
    rdfs:domain :DirectoryDestination ;
    rdfs:range xsd:string .

:DatasetDestination a owl:Class ;
    rdfs:subClassOf :Destination ;
    :inputType :RDFMessage ;
    dct:title "Dataset Destination"@en ;
    dct:description "A DatasetDestination provides configurations for ingesting RDF data into a Mobi Dataset"@en .

# Message

:Messsage a owl:Class ;
    dct:title "Message"@en ;
    dct:description "A Messsage indicates the format of the data flowing through a Workflow at a particular moment."@en .

:previousMessage a owl:ObjectProperty, owl:FunctionalProperty ;
    dct:title "previous message"@en ;
    dct:description "The Message that immediately preceeded the described Message."@en ;
    rdfs:domain :Message ;
    rdfs:range :Message .

:SerializableMessage a owl:Class ;
    rdfs:subClassOf :Message ;
    dct:title "Serializable Message"@en ;
    dct:description "A Message whose contents can be serialized and saved into a file."@en .

:RDFMessage a owl:Class ;
    rdfs:subClassOf :SerializableMessage ;
    dct:title "RDF Message"@en ;
    dct:description "An RDFMessage points to RDF data passing through a Workflow at a particular moment."@en .

:FileMessage a owl:Class ;
    rdfs:subClassOf :Message ;
    dct:title "File Message"@en ;
    dct:description "A FileMessage points to a file passing through a Workflow at a particular moment."@en .

:fileURI a owl:DatatypeProperty ;
    dct:title "file URI"@en ;
    dct:description "The URI of where to retrieve the file represented by the described FileMessage."@en ;
    rdfs:domain :FileMessage ;
    rdfs:range xsd:string .

:fileName a owl:DatatypeProperty ;
    dct:title "file name"@en ;
    dct:description "The name of the file represented by the described FileMessage."@en ;
    rdfs:domain :FileMessage ;
    rdfs:range xsd:string .

:TikaMessage a owl:Class ;
    rdfs:subClassOf :RDFMessage, :FileMessage ;
    dct:title "A TikaMessage points to RDF of Tika generated metadata about a file and the string contents of the file."@en .

# Misc.

:inputType a owl:AnnotationProperty, owl:FunctionalProperty ;
    dct:title "input type"@en ;
    dct:description "The type of Message that the described Destination or Processor expects to receive. The inputType of a Processor or Destination must match the outputType of the parent DataSource or Processor."@en .

:outputType a owl:AnnotationProperty, owl:FunctionalProperty ;
    dct:title "output type"@en ;
    dct:description "The type of Message that the described DataSource or Processor outputs. The outputType of a Processor or DataSource must match the inputType of the parent Processor or Destination."@en .

:filePath a owl:DatatypeProperty, owl:FunctionalProperty ;
    dct:title "file path"@en ;
    dct:description "The string file path to the file of a FileDataSource or FileDestination or the directory of a DirectoryDataSource or DirectoryDestination."@en ;
    rdfs:domain [
        a owl:Class ;
        owl:unionOf ( :FileDataSource :DirectoryDataSource :FileDestination :DirectoryDestination )
    ] ;
    rdfs:range xsd:string .

:datasetRecord a owl:ObjectProperty, owl:FunctionalProperty ;
    dct:title "dataset record"@en ;
    dct:description "The DatasetRecord that the described DatasetDestination uses to ingest data or the described UnstructuredProcessor pulls entity information from."@en ;
    rdfs:domain [
        a owl:Class ;
        owl:unionOf ( :UnstructuredProcessor :DatasetDestination )
        ] ;
    rdfs:range dataset:DatasetRecord .

:append a owl:DatatypeProperty, owl:FunctionalProperty ;
    dct:title "append"@en ;
    dct:description "Whether or not the described FileDestination or DirectoryDestination should append incoming message to a file instead of overwriting it. Default is false."@en ;
    rdfs:domain [
        a owl:Class ;
        owl:unionOf ( :FileDestination :DirectoryDestination )
    ] ;
    rdfs:range xsd:boolean .

:mimeType a owl:DatatypeProperty, owl:FunctionalProperty ;
    dct:title "MIME type"@en ;
    dct:description "A string representing a MIME type. For FileDestinations and DirectoryDestinations, this is the type file will be stored as. For FileMessages, this is the type of the referenced file."@en ;
    rdfs:domain [
        a owl:Class ;
        owl:unionOf ( :FileDestination :DirectoryDestination :FileMessage )
    ] ;
    rdfs:range xsd:string .

:batchSize a owl:DatatypeProperty, owl:FunctionalProperty ;
    dct:title "batch size"@en ;
    dct:description "The number of rows per batch to be processed by the described MappingProcessor or statements per batch to be processed by the described DatasetDestination. Default value is 0 for rows, which means they will be processed one at a time. Default value is 10,000 for statements."@en ;
    rdfs:domain [
        a owl:Class ;
        owl:unionOf ( :MappingProcessor :DatasetDestination )
    ] ;
    rdfs:range xsd:integer .