@prefix owl: <http://www.w3.org/2002/07/owl#>.
@prefix dc: <http://purl.org/dc/elements/1.1/> .
@prefix xsd: <http://www.w3.org/2001/XMLSchema#> .
@prefix rdf: <http://www.w3.org/1999/02/22-rdf-syntax-ns#> .
@prefix rdfs: <http://www.w3.org/2000/01/rdf-schema#> .
@prefix foaf: <http://xmlns.com/foaf/0.1/>.
@prefix dct: <http://purl.org/dc/terms/>.
@prefix : <http://mobi.com/ontologies/federation#> .
@base <http://mobi.com/ontologies/federation>.

<http://mobi.com/ontologies/federation> a owl:Ontology ;
    owl:versionIRI <http://mobi.com/ontologies/federation#2.0>;
    rdfs:label "Mobi Federation Ontology"@en ;
    rdfs:comment "Ontology defining the structures representing federation topologies in Mobi."@en ;
    dct:creator [foaf:name "Sean Smitz"], [foaf:name "Megan Mercer"];
    foaf:maker [foaf:name "Mobi"; foaf:homepage <http://mobi.com>];
    dct:modified "2017-10-04"^^xsd:date.

:Federation a owl:Class ;
    rdfs:label "Mobi Federation"@en ;
    rdfs:comment "A group of locally federated Mobi nodes."@en .

:federationId a rdf:Property , owl:DatatypeProperty , owl:FunctionalProperty ;
    rdfs:domain :Federation ;
    rdfs:range xsd:string ;
    rdfs:label "Federation ID"@en ;
    rdfs:comment "The Federation ID."@en .

:memberNode a rdf:Property , owl:ObjectProperty ;
  rdfs:domain :Federation ;
  rdfs:range :FederationNode ;
  rdfs:label "Member Node"@en ;
  rdfs:comment "Indicates the specified FederationNode is a member of this Federation."@en .

:Node a owl:Class ;
  rdfs:label "Mobi Node"@en ;
  rdfs:comment "A Mobi node, whether local or remote"@en .

:nodeId a rdf:Property , owl:DatatypeProperty , owl:FunctionalProperty ;
  rdfs:domain :Node ;
  rdfs:range xsd:string ;
  rdfs:label "Node ID"@en ;
  rdfs:comment "The ID of the remote node."@en .

:host a rdf:Property , owl:DatatypeProperty , owl:FunctionalProperty ;
  rdfs:domain :Node ;
  rdfs:range xsd:string ;
  rdfs:label "Node Address"@en ;
  rdfs:comment "The network address of the remote node."@en .

:nodeLastUpdated a rdf:Property , owl:DatatypeProperty , owl:FunctionalProperty ;
  rdfs:domain :Node ;
  rdfs:range xsd:dateTime ;
  rdfs:label "Node Last Updated"@en ;
  rdfs:comment "The date and time the node was last updated."@en .

:FederationNode a owl:Class ;
  rdfs:subClassOf :Node ;
  rdfs:label "Local Pod Mobi Node"@en ;
  rdfs:comment "A Mobi node within the local Federation."@en .

:nodeActive a rdf:Property , owl:DatatypeProperty , owl:FunctionalProperty ;
  rdfs:domain :FederationNode ;
  rdfs:range xsd:boolean ;
  rdfs:label "Node Active"@en ;
  rdfs:comment "Whether or not a node is actively part of the federation at a given time"@en .

:membership a rdf:Property, owl:ObjectProperty, owl:FunctionalProperty ;
  rdfs:domain :FederationNode ;
  rdfs:range :FederationMembership ;
  rdfs:label "Membership"@en ;
  rdfs:comment "This node's membership status in the federation."@en .

:gateway a rdf:Property, owl:DatatypeProperty ;
  rdfs:domain :FederationNode ;
  rdfs:range xsd:string ;
  rdfs:label "Gateway"@en ;
  rdfs:comment "The ID of the federation to which this node acts as a gateway."@en .


:FederationMembership owl:EquivalentClass [
  a owl:Class ;
  owl:oneOf ( :full :remote )
] .

:full a :FederationMembership ;
  rdfs:label "FULL"@en ;
  rdfs:comment "A node in the federation which has FULL node access to the federation."@en .

:remote a :FederationMembership ;
  rdfs:label "REMOTE"@en ;
  rdfs:comment "A node in the federation which only has REMOTE node access to the federation."@en .

_:isGateway a [
  a owl:Restriction ;
  owl:minQualifiedCardinality "1"^^xsd:nonNegativeInteger ;
  owl:onProperty :gateway ;
  owl:onClass :FederationNode
] .
