@prefix owl: <http://www.w3.org/2002/07/owl#>.
@prefix foaf: <http://xmlns.com/foaf/0.1/>.
@prefix xsd: <http://www.w3.org/2001/XMLSchema#>.
@prefix rdfs: <http://www.w3.org/2000/01/rdf-schema#>.
@prefix dct: <http://purl.org/dc/terms/>.
@prefix sh: <http://www.w3.org/ns/shacl#>.
@prefix um: <http://mobi.com/ontologies/user/management#>.
@prefix pref: <http://mobi.com/ontologies/preference#>.
@prefix : <http://mobi.com/ontologies/notification#>.
@base <http://mobi.com/ontologies/notification>.

<http://mobi.com/ontologies/notification> a owl:Ontology;
    owl:versionIRI <http://mobi.com/ontologies/notification/1.0>;
    owl:imports <http://www.w3.org/ns/shacl#>, <http://mobi.com/ontologies/preference>;
    rdfs:label "The Notification Preference Shape Ontology"@en;
    rdfs:comment "The Notification Preference Shape Ontology provides the SHACL shapes relating to Notification Preferences."@en;
    dct:creator [foaf:name "Ben Greenberg"];
    foaf:maker [foaf:name "Mobi"; foaf:homepage <https://mobi.inovexcorp.com/>];
    dct:modified "2020-12-15"^^xsd:date.

:EmailNotificationPreference a owl:Class, sh:NodeShape;
    rdfs:subClassOf pref:Preference;
    rdfs:label "Email Notifications"@en;
    rdfs:comment "A preference that a user can have within the Mobi framework that signifies whether they want to receive email notifications."@en;
    sh:property :EmailNotificationPreferencePropertyShape;
    pref:inGroup :NotificationPreferenceGroup .

:EmailNotificationPreferencePropertyShape a sh:PropertyShape;
    rdfs:label "Would you like to receive Email Notifications?"@en;
    sh:path pref:hasDataValue;
    sh:datatype xsd:boolean;
    sh:in ( "yes" "no" ) ;
    sh:minCount 1 ;
    sh:maxCount 1 ;
    pref:usesFormField pref:RadioInput .

:SomeSimpleTextPreference a owl:Class, sh:NodeShape;
    rdfs:subClassOf pref:Preference;
    rdfs:label "Email Notification Preference"@en;
    rdfs:comment "A preference that a user can have within the Mobi framework that signifies whether they want to receive email notifications."@en;
    sh:property :SomeSimpleTextPreferencePropertyShape;
    pref:inGroup :NotificationPreferenceGroup .

:SomeSimpleTextPreferencePropertyShape a sh:PropertyShape;
    sh:path pref:hasDataValue;
    sh:datatype xsd:string;
    sh:minCount 1 ;
    sh:maxCount 2 ;
    pref:usesFormField pref:TextInput .

:NotificationPreferenceGroup a pref:PreferenceGroup ;
    rdfs:label "Notifications"@en .

:PrefixPreference a owl:Class, sh:NodeShape;
    rdfs:subClassOf pref:Preference;
    rdfs:label "Prefix Preference"@en;
    rdfs:comment "A preference that a user can have within the Mobi framework that signifies the prefixes they want defined."@en;
    sh:property :PrefixPreferencePropertyShape;
    pref:inGroup :PrefixPreferenceGroup .

:PrefixPreferenceGroup a pref:PreferenceGroup .

:PrefixPreferencePropertyShape a sh:PropertyShape;
    sh:node :PrefixNodeShape;
    sh:path pref:hasObjectValue .

:PrefixNodeShape a sh:NodeShape;
    sh:property :PrefixPropertyShape;
    sh:property :NamespacePropertyShape;
    sh:targetClass :Prefix .

:PrefixPropertyShape a sh:PropertyShape ;
    sh:path :hasPrefix ;
    sh:datatype xsd:string ;
    sh:order 0 ;
    sh:minCount 1 ;
    sh:maxCount 1 ;
    pref:usesFormField pref:TextInput .

:NamespacePropertyShape a sh:PropertyShape ;
    sh:path :hasNamespace ;
    sh:datatype xsd:string ;
    sh:pattern "((([A-Za-z]{3,9}:(?:\/\/)?)(?:[-;:&=\+\$,\w]+@)?[A-Za-z0-9.-]+(:[0-9]+)?|(?:www.|[-;:&=\+\$,\w]+@)[A-Za-z0-9.-]+)((?:\/[\+~%\/.\w-_]*)?\??(?:[-\+=&;%@.\w_]*)#?(?:[\w]*))?)" ;
    sh:order 1 ;
    sh:minCount 1 ;
    sh:maxCount 1 ;
    pref:usesFormField pref:TextInput .

:Prefix a owl:Class;
    rdfs:label "Prefix"@en.

:hasPrefix a owl:DatatypeProperty, owl:FunctionalProperty;
   rdfs:label "Has Prefix"@en;
   rdfs:domain :Prefix;
   rdfs:range xsd:string .

:hasNamespace a owl:DatatypeProperty, owl:FunctionalProperty;
   rdfs:label "Has Namespace"@en;
   rdfs:domain :Prefix;
   rdfs:range xsd:string .