@prefix rdf: <http://www.w3.org/1999/02/22-rdf-syntax-ns#> .
@prefix rdfs: <http://www.w3.org/2000/01/rdf-schema#> .
@prefix owl: <http://www.w3.org/2002/07/owl#> .
@prefix xsd: <http://www.w3.org/2001/XMLSchema#> .
@prefix foaf: <http://xmlns.com/foaf/0.1/> .
@prefix dct: <http://purl.org/dc/terms/> .
@prefix prov: <http://www.w3.org/ns/prov-o#> .
@prefix matg: <http://mobi.com/ontologies/graph#> .
@prefix matcat: <http://mobi.com/ontologies/catalog#> .
@prefix mobi: <http://mobi.com/ontologies/mobi#> .
@prefix : <http://mobi.com/ontologies/dataset#> .
@base <http://mobi.com/ontologies/dataset> .

<http://mobi.com/ontologies/dataset> a owl:Ontology ;
    owl:versionIRI <http://mobi.com/ontologies/dataset#1.0> ;
    owl:imports <http://mobi.com/ontologies/catalog> , <http://mobi.com/ontologies/Mobi> ;
    rdfs:label "Mobi Dataset Ontology"@en;
    rdfs:comment "The Mobi dataset ontology describes the structure of dataset objects and how they relate to the Mobi Catalog."@en;
    dct:creator [foaf:name "Stephen Kahmann"] ;
    foaf:maker [foaf:name "Mobi" ; foaf:homepage <https://mobi.inovexcorp.com/>] ;
    dct:modified "2017-10-06"^^xsd:date .

# Dataset

:Dataset a owl:Class ;
    rdfs:label "Dataset"@en ;
    rdfs:comment "A collection of named graph identifiers that correspond to RDF Graphs in an RDF Dataset."@en ;
    rdfs:seeAlso "https://www.w3.org/TR/rdf11-concepts/#section-dataset" .

:systemDefaultNamedGraph a owl:ObjectProperty , owl:FunctionalProperty ;
    rdfs:label "System Default Named Graph"@en ;
    rdfs:comment "The resource representing the default named graph of an RDF Dataset that is created and maintained
    by the system. This graph is used when loading default graph data and no other default named graph is specified"@en ;
    rdfs:seeAlso "https://www.w3.org/TR/rdf11-concepts/#section-dataset" ;
    rdfs:domain :Dataset ;
    rdfs:range mobi:Identifier .

:defaultNamedGraph a owl:ObjectProperty ;
    rdfs:label "Default Named Graph"@en ;
    rdfs:comment "A resource representing a default named graph of an RDF Dataset."@en ;
    rdfs:seeAlso "https://www.w3.org/TR/rdf11-concepts/#section-dataset" ;
    rdfs:domain :Dataset ;
    rdfs:range mobi:Identifier .

:namedGraph a owl:ObjectProperty ;
    rdfs:label "Named Graph"@en ;
    rdfs:comment "A resource representing a named graph of an RDF Dataset."@en ;
    rdfs:seeAlso "https://www.w3.org/TR/rdf11-concepts/#section-dataset" ;
    rdfs:domain :Dataset ;
    rdfs:range mobi:Identifier .

# DatasetRecord

:DatasetRecord a owl:Class ;
    rdfs:subClassOf matcat:UnversionedRecord ;
    rdfs:label "Dataset"@en ;
    rdfs:comment "A record describing a collection of RDF Graphs that make up an RDF Dataset."@en ;
    rdfs:seeAlso "https://www.w3.org/TR/rdf11-concepts/#section-dataset" .

:dataset a owl:ObjectProperty , owl:FunctionalProperty ;
    rdfs:label "Dataset"@en ;
    rdfs:comment "The Dataset described by this record."@en ;
    rdfs:seeAlso "https://www.w3.org/TR/rdf11-concepts/#section-dataset" ;
    rdfs:domain :DatasetRecord ;
    rdfs:range :Dataset .

:repository a owl:DatatypeProperty , owl:FunctionalProperty ;
    rdfs:label "Repository"@en ;
    rdfs:comment "The repository where the dataset object and its data is stored."@en ;
    rdfs:domain :DatasetRecord ;
    rdfs:range xsd:string .

:ontology a owl:DatatypeProperty ;
    rdfs:domain :DatasetRecord .

# Misc.

:linksToRecord a owl:ObjectProperty, owl:FunctionalProperty ;
    rdfs:range matcat:VersionedRDFRecord .

:linksToBranch a owl:ObjectProperty, owl:FunctionalProperty ;
    rdfs:range matcat:Branch .

:linksToCommit a owl:ObjectProperty, owl:FunctionalProperty ;
    rdfs:range matcat:Commit .