@prefix rdf: <http://www.w3.org/1999/02/22-rdf-syntax-ns#> .
@prefix rdfs: <http://www.w3.org/2000/01/rdf-schema#> .
@prefix owl: <http://www.w3.org/2002/07/owl#> .
@prefix xsd: <http://www.w3.org/2001/XMLSchema#> .
@prefix foaf: <http://xmlns.com/foaf/0.1/> .
@prefix dct: <http://purl.org/dc/terms/> .
@prefix prov: <http://www.w3.org/ns/prov-o#> .
@prefix matg: <http://matonto.org/ontologies/graph#> .
@prefix matcat: <http://matonto.org/ontologies/catalog#> .
@prefix : <http://matonto.org/ontologies/dataset#> .
@base <http://matonto.org/ontologies/dataset> .

<http://matonto.org/ontologies/dataset> a owl:Ontology ;
    owl:versionIRI <http://matonto.org/ontologies/dataset#1.0> ;
    owl:imports <http://matonto.org/ontologies/catalog> ;
    rdfs:label "MatOnto Dataset Ontology"@en;
    rdfs:comment "The MatOnto dataset ontology describes the structure of dataset objects and how they relate to the MatOnto Catalog."@en;
    dct:creator [foaf:name "Stephen Kahmann"] ;
    foaf:maker [foaf:name "MatOnto" ; foaf:homepage <http://matonto.org>] ;
    dct:modified "2017-02-20"^^xsd:date .

# Dataset

:Dataset a owl:Class ;
    rdfs:label "Dataset"@en ;
    rdfs:comment "A collection of named graph identifiers that correspond to RDF Graphs in an RDF Dataset."@en ;
    rdfs:seeAlso "https://www.w3.org/TR/rdf11-concepts/#section-dataset" .

:defaultNamedGraph a owl:ObjectProperty ;
    rdfs:label "Default Named Graph"@en ;
    rdfs:comment "A resource representing a default named graph of an RDF Dataset."@en ;
    rdfs:seeAlso "https://www.w3.org/TR/rdf11-concepts/#section-dataset" ;
    rdfs:domain :Dataset ;
    rdfs:range matg:Graph .

:namedGraph a owl:ObjectProperty ;
    rdfs:label "Named Graph"@en ;
    rdfs:comment "A resource representing a named graph of an RDF Dataset."@en ;
    rdfs:seeAlso "https://www.w3.org/TR/rdf11-concepts/#section-dataset" ;
    rdfs:domain :Dataset ;
    rdfs:range matg:Graph .

# DatasetRecord

:DatasetRecord a owl:Class ;
    rdfs:subClassOf matcat:UnversionedRecord ;
    rdfs:label "Dataset"@en ;
    rdfs:comment "A record describing a collection of RDF Graphs that make up an RDF Dataset."@en ;
    rdfs:seeAlso "https://www.w3.org/TR/rdf11-concepts/#section-dataset" .

:dataset a owl:ObjectProperty , owl:FunctionalProperty ;
    rdfs:label "Dataset"@en ;
    rdfs:comment "The Dataset described by this record."@en ;
    rdfs:seeAlso "https://www.w3.org/TR/rdf11-concepts/#section-dataset" ;
    rdfs:domain :DatasetRecord ;
    rdfs:range :Dataset .
