@prefix owl: <http://www.w3.org/2002/07/owl#> .
@prefix rdfs: <http://www.w3.org/2000/01/rdf-schema#> .
@prefix xsd: <http://www.w3.org/2001/XMLSchema#> .
@prefix dc: <http://purl.org/dc/elements/1.1/> .
@prefix dct: <http://purl.org/dc/terms/>.
@prefix : <urn://mobi.com/ontologies/MeaningExtraction#> .

<urn://mobi.com/ontologies/MeaningExtraction> a owl:Ontology ;
    owl:versionIRI <urn://mobi.com/ontologies/MeaningExtraction#1.0> ;
    rdfs:label "Mobi Extraction Ontology"@en ;
    rdfs:comment "Ontology extension for generating ontologies ."@en ;
    dct:creator [foaf:name "Ben Gould"] ;
    foaf:maker [foaf:name "Mobi"; foaf:homepage <http://mobi.com>] ;
    dct:modified "2017-12-01"^^xsd:date .

##########################################
##########################################

:ExtractedOntology a owl:Class ;
    rdfs:subClassOf owl:Ontology ;
    rdfs:label "Extracted Ontology"@en ;
    rdfs:comment "Ontology generated by extracting meaning from files"@en .

:spelClassUri a rdf:Property , owl:DatatypeProperty , owl:FunctionalProperty ;
    rdfs:domain :ExtractedOntology ;
    rdfs:range xsd:string ;
    rdfs:label "Property URI Expression"@en ;
    rdfs:comment "Spring Expression Language template for generating URIs for properties discovered from the meaning extraction APIs."@en .

:spelPropertyUri a rdf:Property , owl:DatatypeProperty , owl:FunctionalProperty ;
    rdfs:domain :ExtractedOntology ;
    rdfs:range xsd:string ;
    rdfs:label "Class URI Expression"@en ;
    rdfs:comment "Spring Expression Language template for generating URIs for classes discovered from the meaning extraction APIs."@en .

##########################################

:ExtractedClass a owl:Class ;
    rdfs:subClassOf owl:Class ;
    rdfs:label "Extracted Class"@en ;
    rdfs:comment "Class extracted from the meaning extraction APIs."@en .

:spelInstanceUri a rdf:Property , owl:DatatypeProperty , owl:FunctionalProperty ;
    rdfs:domain :ExtractedClass ;
    rdfs:range xsd:string ;
    rdfs:label "Instance URI Expression"@en ;
    rdfs:comment "Spring Expression Language template for generating URIs for instances of this class discovered from the meaning extraction APIs."@en .

##########################################

:ExtractedProperty a owl:Class ;
    rdfs:subClassOf rdf:Property ;
    rdfs:label "Extracted Property"@en ;
    rdfs:comment "Property extracted from the meaning extraction APIs."@en .

##########################################

:ExtractedDatatypeProperty a owl:Class ;
    rdfs:subClassOf owl:DatatypeProperty , :ExtractedProperty ;
    rdfs:label "Extracted Data Type Property"@en ;
    rdfs:comment "Data Type Property extracted from the meaning extraction APIs."@en .

##########################################

:ExtractedObjectProperty a owl:Class ;
    rdfs:subClassOf owl:ObjectProperty , :ExtractedProperty ;
    rdfs:label "Extracted Object Property"@en ;
    rdfs:comment "Object Property extracted from the meaning extraction APIs."@en .
