@prefix rdf: <http://www.w3.org/1999/02/22-rdf-syntax-ns#>.
@prefix owl: <http://www.w3.org/2002/07/owl#>.
@prefix dc: <http://purl.org/dc/elements/1.1/>.
@prefix xsd: <http://www.w3.org/2001/XMLSchema#>.
@prefix foaf: <http://xmlns.com/foaf/0.1/>.
@prefix rdfs: <http://www.w3.org/2000/01/rdf-schema#>.
@prefix dct: <http://purl.org/dc/terms/>.
@prefix prov: <http://www.w3.org/ns/prov#>.
@prefix : <http://matonto.org/ontologies/versioning#>.
@base <http://matonto.org/ontologies/versioning#>.

<http://matonto.org/ontologies/versioning> a owl:Ontology;
    owl:versionIRI <http://matonto.org/ontologies/versioning/1.1>;
    owl:imports <http://www.w3.org/ns/prov#>;
    rdfs:label "The MatOnto Versioning Ontology"@en;
    rdfs:comment "The MatOnto versioning ontology describes how versioning is handled within the MatOnto framework."@en;
    dct:creator [foaf:name "Jordan Lewis"];
    foaf:maker [foaf:name "MatOnto"; foaf:homepage <http://matonto.org>];
    dct:modified "2016-10-05"^^xsd:date.

# Commit

:Commit a owl:Class;
    rdfs:subClassOf prov:Activity;
    rdfs:label "Commit"@en;
    rdfs:comment "The provenance describing a commit activity made on a Resource."@en.

# In Progress Commit

:InProgressCommit a owl:Class;
    rdfs:subClassOf :Commit;
    rdfs:label "In Progress Commit"@en;
    rdfs:comment "The provenance describing a commit activity that is currently being made on a Resource."@en.

# Revision

:Revision a owl:Class;
    rdfs:subClassOf prov:Entity;
    rdfs:label "Revision"@en;
    rdfs:comment "The entity created by a user's Commit."@en.

:additions a owl:ObjectProperty, owl:FunctionalProperty;
    rdfs:label "additions"@en;
    rdfs:comment "Links the IRI of a graph containing the statements that were added with the described Revision."@en;
    rdfs:domain :Revision;
    rdfs:range rdfs:Resource.

:deletions a owl:ObjectProperty, owl:FunctionalProperty;
    rdfs:label "deletions"@en;
    rdfs:comment "Links the IRI of a graph containing the statements that were deleted with the described Revision."@en;
    rdfs:domain :Revision;
    rdfs:range rdfs:Resource.
